SetTheory/Basic.lean
@@ -6,59 +6,53 @@ Development roughly follows *(Introduction to Set Theory* by Karel Hrbacek and T
 
 namespace SetTheory
 
-variable [MorseKelley M] {x y z : M}
+variable [Zermelo V] {x y z : V}
 
-theorem left_mem_pair : IsSet x → IsSet y → x ∈ pair x y :=
-  by aesop
+theorem left_mem_pair : x ∈ pair x y :=
+  by simp
 
-theorem right_mem_pair : IsSet x → IsSet y → x ∈ pair x y :=
-  by aesop
+theorem right_mem_pair : y ∈ pair x y :=
+  by simp
 
 @[simp]
 theorem pair_self : pair x x = {x} :=
   rfl
 
-@[aesop safe]
-theorem pair_nonemptyClass : IsSet x → IsSet y → NonemptyClass (pair x y) :=
-  fun hx hy => ⟨x, left_mem_pair hx hy⟩
+@[simp]
+theorem pair_nonemptyClass : NonemptySet (pair x y) :=
+  ⟨x, left_mem_pair⟩
 
-/-- The intersection of a set `x`. Constructed as the class `{y | ∀ t, t ∈ x → y ∈ t}`. -/
-def sInter (x : M) : M :=
-  ofFormula (.all (.imp
+/-- The intersection of a set `x`. Constructed as the set `{y ∈ ⋃ x | ∀ t, t ∈ x → y ∈ t}`. -/
+def sInter (x : V) : V :=
+  sep
+  (.all (.imp
     (.mem (Sum.inr 1) (Sum.inl ()))
     (.mem (Sum.inr 0) (Sum.inr 1))))
   (fun (_ : Unit) => x)
+  (⋃ x)
 
 /-- We will use the notation `⋂` for set intersection in this project. -/
 prefix:110 "⋂ " => sInter
 
-@[aesop norm]
-theorem mem_sInter_iff (hx : NonemptyClass x) :
-    y ∈ ⋂ x ↔ ∀ t ∈ x, y ∈ t := by
-  unfold sInter
-  simp
-  intro h
-  obtain ⟨z, hz⟩ := hx
-  exact ⟨z, h z hz⟩
+@[simp]
+theorem mem_sInter_iff :
+    y ∈ ⋂ x ↔ NonemptySet x ∧ ∀ t ∈ x, y ∈ t := by
+  unfold sInter NonemptySet
+  aesop
 
-theorem subset_sInter : NonemptyClass x → y ∈ x → ⋂ x ⊆ y := by
+theorem subset_sInter : NonemptySet x → y ∈ x → ⋂ x ⊆ y := by
   intro hx h z hz
   aesop
 
-theorem sInter_isSet (hx : NonemptyClass x) : IsSet (⋂ x) := by
-  obtain ⟨y, hy⟩ := hx
-  refine subset_isSet (subset_sInter ⟨y, hy⟩ hy) ⟨x, hy⟩
-
 /-- The intersection of two sets `x` and `y`. -/
-instance : Inter M where
-  inter x y := sInter (pair x y)
+instance : Inter V where
+  inter x y := ⋂ pair x y
 
 @[simp]
-theorem mem_inter_iff (hx : IsSet x) (hy : IsSet y) :
+theorem mem_inter_iff :
     z ∈ x ∩ y ↔ z ∈ x ∧ z ∈ y := by
-  show z ∈ sInter (pair x y) ↔ z ∈ x ∧ z ∈ y
-  rw [mem_sInter_iff (pair_nonemptyClass hx hy)]
-  aesop
+  show z ∈ ⋂ pair x y ↔ z ∈ x ∧ z ∈ y
+  simp
 
 @[simp]
 theorem sUnion_pair : ⋃ pair x y = x ∪ y := rfl
@@ -66,46 +60,32 @@ theorem sUnion_pair : ⋃ pair x y = x ∪ y := rfl
 @[simp]
 theorem sInter_pair : ⋂ pair x y = x ∩ y := rfl
 
-/-- The axiom scheme of *separation*. -/
-def sep (p : BoundedFormula α 1) (v : α → M) (x : M) : M :=
-  ofFormula (
-    (p.sum Unit).and
-    (.mem (Sum.inr 0) (Sum.inl (Sum.inr ()))))
-  (Sum.elim v (fun _ => x))
+@[simp]
+theorem union_self : x ∪ x = x :=
+  by ext; simp
 
 @[simp]
-theorem mem_sep_iff : x ∈ sep p v y ↔ x ∈ y ∧ Interpret M p v (fun _ => x) := by
-  unfold sep
-  aesop
+theorem inter_self : x ∩ x = x :=
+  by ext; simp
 
-@[simp]
-theorem union_self (hx : IsSet x) : x ∪ x = x :=
-  by ext; aesop
-
-@[simp]
-theorem inter_self (hx : IsSet x) : x ∩ x = x :=
-  by ext; aesop
-
-theorem union_pair_eq_inter_pair (hx : IsSet x) (hy : IsSet y) :
+theorem union_pair_eq_inter_pair :
     {x} ∪ pair x y = {x} ∩ pair x y ↔ x = y := by
   constructor
   · intro h
     rw [ext_iff] at h
     have := (h y).mp ?_
-    · rw [mem_inter_iff (singleton_isSet hx) (pair_isSet hx hy),
-        mem_singleton_iff hx] at this
+    · rw [mem_inter_iff, mem_singleton_iff] at this
       exact this.1.symm
-    · rw [mem_union_iff (singleton_isSet hx) (pair_isSet hx hy)]
-      aesop
+    · simp
   · rintro rfl
-    simp [union_self (singleton_isSet hx), inter_self (singleton_isSet hx)]
+    simp
 
 /-- The first projection of a Kuratowski ordered pair. -/
-def π₁ (x : M) : M :=
+def π₁ (x : V) : V :=
   ⋃ ⋂ x
 
 /-- The second projection of a Kuratowski ordered pair. -/
-def π₂ (x : M) : M :=
+def π₂ (x : V) : V :=
   ⋃ sep
     (.imp
       (.ne (Sum.inl true) (Sum.inl false))
@@ -117,103 +97,38 @@ theorem mem_π₂_iff : y ∈ π₂ x ↔ ∃ z, y ∈ z ∧ z ∈ ⋃ x ∧ (�
   aesop
 
 @[simp]
-theorem π₁_opair (hx : IsSet x) (hy : IsSet y) : π₁ (opair x y) = x := by
+theorem π₁_opair : π₁ (opair x y) = x := by
   unfold π₁ opair
   ext z
-  simp [mem_inter_iff (singleton_isSet hx) (pair_isSet hx hy)]
   aesop
 
 @[simp]
-theorem π₂_opair (hx : IsSet x) (hy : IsSet y) : π₂ (opair x y) = y := by
+theorem π₂_opair : π₂ (opair x y) = y := by
   unfold opair
   ext z
   rw [mem_π₂_iff]
-  simp only [sUnion_pair, sInter_pair, ne_eq, union_pair_eq_inter_pair hx hy]
+  simp only [sUnion_pair, sInter_pair, ne_eq, union_pair_eq_inter_pair]
   constructor
   · rintro ⟨s, hzs, hsx, hs⟩
     by_cases h : s = y
     · subst h
       exact hzs
-    rw [mem_union_iff (singleton_isSet hx) (pair_isSet hx hy),
-      mem_singleton_iff hx] at hsx
-    cases hsx with
-    | inl hsx =>
-      subst hsx
-      exfalso
-      refine hs h ?_
-      rw [mem_inter_iff (singleton_isSet hx) (pair_isSet hx hy)]
-      aesop
-    | inr hsx =>
-      rw [mem_pair_iff hx hy] at hsx
-      cases hsx with
-      | inl hsx =>
-        subst hsx
-        exfalso
-        refine hs h ?_
-        rw [mem_inter_iff (singleton_isSet hx) (pair_isSet hx hy)]
-        aesop
-      | inr hsx =>
-        subst hsx
-        exact hzs
-  · intro hzy
-    refine ⟨y, hzy, ?_, ?_⟩
-    · rw [mem_union_iff (singleton_isSet hx) (pair_isSet hx hy),
-        mem_pair_iff hx hy]
-      exact Or.inr (Or.inr rfl)
-    · intro h
-      refine (fun h' => h ?_)
-      rw [mem_inter_iff (singleton_isSet hx) (pair_isSet hx hy)] at h'
-      aesop
+    · aesop
+  · aesop
 
 @[simp]
-theorem opair_injective {x y z w : M} (hx : IsSet x) (hy : IsSet y) (hz : IsSet z) (hw : IsSet w) :
+theorem opair_injective {x y z w : V} :
     opair x y = opair z w ↔ x = z ∧ y = w := by
   constructor
   · intro h
     have h₁ := congrArg π₁ h
     have h₂ := congrArg π₂ h
-    simp [π₁_opair hx hy, π₁_opair hz hw] at h₁
-    simp [π₂_opair hx hy, π₂_opair hz hw] at h₂
+    simp at h₁ h₂
     exact ⟨h₁, h₂⟩
   · rintro ⟨rfl, rfl⟩
     rfl
 
 theorem forall_not_mem (h : ∀ y, y ∉ x) : x = ∅ :=
   by ext; aesop
-
-theorem subset_univ : x ⊆ univ :=
-  by intro; aesop
-
-def russellClass : M :=
-  ofFormula (.not (.mem (Sum.inr 0) (Sum.inr 0))) (fun (i : Empty) => i.elim)
-
-@[simp]
-theorem mem_russellClass_iff :
-    x ∈ (russellClass : M) ↔ IsSet x ∧ x ∉ x := by
-  unfold russellClass
-  simp
-
-theorem russellClass_not_mem (h : russellClass ∈ (russellClass : M)) :
-    russellClass ∉ (russellClass : M) := by
-  rw [mem_russellClass_iff] at h
-  exact h.2
-
-theorem russellClass_mem
-    (h₁ : IsSet (russellClass : M)) (h₂ : russellClass ∉ (russellClass : M)) :
-    russellClass ∈ (russellClass : M) := by
-  rw [mem_russellClass_iff, not_and, not_not] at h₂
-  exact h₂ h₁
-
-/-- The Russell class is not a set. -/
-theorem russellClass_not_isSet : ¬IsSet (russellClass : M) := by
-  intro h
-  by_cases h' : russellClass ∈ (russellClass : M)
-  · exact russellClass_not_mem h' h'
-  · exact h' (russellClass_mem h h')
-
-/-- The universe is not a set. -/
-theorem univ_not_isSet : ¬IsSet (univ : M) := by
-  intro h
-  exact russellClass_not_isSet (subset_isSet subset_univ h)
 
 end SetTheory
