SetTheory/SetTheory.lean
@@ -4,34 +4,21 @@ import Aesop
 # Models of set theory
 -/
 
-/-- M is a *model of set theory* if it has a membership operation.
-Elements of M are called *classes*. -/
-class SetTheory (M : Type _) extends Membership M M
+/-- `V` is a *model of set theory* if it has a membership operation.
+Elements of `V` are called *sets*. -/
+class SetTheory (V : Type _) extends Membership V V
 
 namespace SetTheory
 
-instance [SetTheory M] : HasSubset M where
-  Subset x y := ∀ ⦃z : M⦄, z ∈ x → z ∈ y
+instance [SetTheory V] : HasSubset V where
+  Subset x y := ∀ ⦃z : V⦄, z ∈ x → z ∈ y
 
 @[aesop unsafe 50% apply]
-theorem subset_iff [SetTheory M] (x y : M) : x ⊆ y ↔ ∀ ⦃z : M⦄, z ∈ x → z ∈ y :=
+theorem subset_iff [SetTheory V] (x y : V) : x ⊆ y ↔ ∀ ⦃z : V⦄, z ∈ x → z ∈ y :=
   Iff.rfl
 
-/-- A class is a *set* if it is an element of a class. -/
-def IsSet [SetTheory M] (x : M) : Prop :=
-  ∃ y : M, x ∈ y
-
-@[aesop unsafe 50% apply]
-theorem isSet_of_mem [SetTheory M] {x y : M} (h : x ∈ y) : IsSet x :=
-  ⟨y, h⟩
-
-/-- A *set* in a set theory M is a class that is a set.
-Not to be confused with Mathlib's `Set`. -/
-def Set (M : Type _) [SetTheory M] : Type _ :=
-  {x : M // IsSet x}
-
-/-- A class is *nonempty* if it has an element. -/
-def NonemptyClass [SetTheory M] (x : M) : Prop :=
-  ∃ y : M, y ∈ x
+/-- A set is *nonempty* if it has an element. -/
+def NonemptySet [SetTheory V] (x : V) : Prop :=
+  ∃ y : V, y ∈ x
 
 end SetTheory
